Working on counter examples for the reifier.

examples/PolyApply/Test.v
@@ -10,9 +10,16 @@ Require Import MirrorCore.PLemma.
 Require Import MirrorCore.Polymorphic.
 Require Import MirrorCore.Lambda.RewriteRelations.
 Require Import MirrorCore.ExprI.
+Require Import MirrorCore.CTypes.CoreTypes.
 
 Inductive my_forall (typ : Set) : Set :=
-| MyForall (t : typ).
+| MyForall (t : typ)
+| MyEq (t : typ)
+| MyImpl
+| MyTrue.
+
+Inductive my_types : nat -> Set :=
+| MyNat : my_types 0.
 
 Section MakeILogic.
   Context {typ func : Set} {FV : PartialView func (my_forall typ)}.
@@ -22,6 +29,72 @@ Section MakeILogic.
   Definition mkForall (t : typ) (f : expr typ func) := App (Inj (fForall t)) (Abs t f).
 
 End MakeILogic.
+
+Definition IgnorePatterns (ls : list RPattern) (T : Set) : Set := T.
+Section for_ignore.
+  Variable ls : list RPattern.
+  Variable T : Set.
+ 
+  Definition reify_IgnorePatterns {R : Reify T}
+  : Command T :=
+    let ignores :=
+        map (fun p => CPattern (ls:=(T : Type)::nil) p (fun (a : function (CRec 0)) => a)) ls
+    in
+    CFix (CFirst_ (ignores ++ CCall (@reify_scheme _ R) :: nil)).
+
+  Global Instance Reify_IgnorePatterns {R : Reify T} : Reify (IgnorePatterns ls T) :=
+  { reify_scheme := @reify_IgnorePatterns R }.
+
+End for_ignore.
+
+Arguments reify_IgnorePatterns {_} _ {_}.
+
+Definition typ := ctyp my_types.
+
+Axiom RType_typ : RType typ.
+Axiom Typ2_typ : Typ2 RType_typ Fun.
+Print reify_func_aux.
+Local Instance Reify_typ : Reify typ := 
+  Reify_typ typ ((CPattern (ls := nil) (RExact nat) (tyBase0 MyNat))::nil).
+
+Definition reify_pforall_no_sect : Command@{Set} (expr typ (my_forall typ)) :=
+  CPattern (ls := (typ : Type) :: (expr typ (my_forall typ) : Type) :: nil)
+           (RPi (RGet 0 RIgnore) (RGet 1 RIgnore))
+           (fun (x : function (CCall (reify_scheme typ))) (y : function (CRec 0)) =>
+              (App (Inj (MyForall typ x)) (Abs x y))).
+
+Definition reify_peq_no_sect : Command@{Set} (expr typ (my_forall typ)) :=
+  CPattern (ls := (typ : Type) :: nil)
+           (RApp (RExact (@eq)) (RGet 0 RIgnore))
+           (fun (x : function (CCall (reify_scheme typ))) =>
+              (Inj (MyEq typ x))).
+
+Definition reify_ptrue_no_sect : Command@{Set} (expr typ (my_forall typ)) :=
+  CPattern (ls := nil) (RExact True) (Inj (MyTrue typ)).
+  
+Definition reify_pimpl_no_sect : Command@{Set} (expr typ (my_forall typ)) :=
+  CPattern (ls := (expr typ (my_forall typ) : Type) :: (expr typ (my_forall typ) : Type) :: nil) 
+           (RImpl (RGet 0 RIgnore) (RGet 1 RIgnore))
+           (fun (x y : function (CRec 0)) =>
+              (App (App (Inj (MyImpl typ)) x) y)).
+
+Local Instance Reify_expr_no_sect : Reify (expr typ (my_forall typ)) :=
+  Reify_func_no_table typ (my_forall typ) (reify_pimpl_no_sect :: reify_ptrue_no_sect :: reify_peq_no_sect :: reify_pforall_no_sect :: nil).
+
+Definition reify_poly_no_sect := reify_scheme@{Set} (IgnorePatterns (RImpl (RExact True) (RGet 0 RIgnore)::nil) (expr typ (my_forall typ))).
+  Ltac reify_poly_no_sect e :=
+    let k e :=
+        pose e in
+    reify_expr reify_poly_no_sect k
+               [[ True ]]
+               [[ e ]].
+
+  Goal True.
+    (* This reifies *)
+    reify_poly_no_sect (forall x : nat, True -> x = x).
+    apply I.
+  Qed.
+
 
 Section Test.
   Context {typ func : Set}.
@@ -43,7 +116,6 @@ Section Test.
   Local Instance Reify_typ : Reify typ :=
     Reify_typ typ (reify_base_typ typ :: nil).
 
-
   Definition reify_pforall : Command@{Set} (expr typ func) :=
     CPattern (ls := (typ : Type) :: (expr typ func : Type) :: nil)
              (RPi (RGet 0 RIgnore) (RGet 1 RIgnore))
@@ -54,12 +126,12 @@ Section Test.
   Local Instance Reify_expr : Reify (expr typ func) :=
     Reify_func_no_table typ func (reify_eq typ func :: reify_pforall :: nil).
 
-  Lemma Id {A} : forall P : A, P = P.
+  Lemma Id {A} : forall P : A, True -> P = P.
   Proof.
     reflexivity.
   Qed.
 
-  Definition reify_poly := reify_scheme@{Set} (expr typ func).
+  Definition reify_poly := reify_scheme@{Set} (IgnorePatterns (RImpl (RExact True) (RGet 0 RIgnore)::nil) (expr typ func)).
   Ltac reify_poly e :=
     let k e :=
         pose e in
@@ -69,18 +141,16 @@ Section Test.
 
   Goal True.
     (* This reifies *)
-    reify_poly (forall x : nat, x = x).
+    reify_poly (forall x : nat, True -> x = x).
     apply I.
   Qed.
-    
+
+
 
   Definition lem_landexistsDL : 
-    polymorphic typ 1
+    polymorphic typ 1 (IgnorePatterns (RImpl (RExact True) (RGet 0 RIgnore)::nil)
                 (Lemma.lemma typ (expr typ func) 
-                             (rw_concl typ func (expr typ func))).   
-  Proof.
-    (* But this does not *)
+                             (rw_concl typ func (expr typ func)))) :=
     Eval unfold Lemma.add_var, Lemma.add_prem , Lemma.vars , Lemma.concl , Lemma.premises in
         <:: @Id ::>.
-  Qed.
-    
+Print lem_landexistsDL.    
